Add soundness proof structure and maximal simplification of hasTableau inductive (#25)
Closes: #24 

Simplified everything to get a minimal calculus that is sound.

theories/ATPCompat.v
@@ -764,7 +764,7 @@ Section ValidityEquivalence.
   Section GenTranslationEquivalidity.
     Lemma gen_interp_term_interp_eterm :
       forall (M : Model string string) (t : ETerm) (bvs : list string) (rho : list M) (sigma : env M string),
-      interpret_term rho sigma (translate_ETerm bvs t) =
+      interpret_term M rho sigma (translate_ETerm bvs t) =
         interpret_eterm (extended_environment bvs rho sigma) t.
     Proof.
       intros ?????. induction t using eterm_ind; cbn.
@@ -790,7 +790,7 @@ Section ValidityEquivalence.
 
       (* Cases: predicates *)
       - intros; cbn.
-        have e : map (interpret_term rho sigma) (map (translate_ETerm bvs) l) =
+        have e : map (interpret_term M rho sigma) (map (translate_ETerm bvs) l) =
                    map (interpret_eterm (extended_environment bvs rho sigma)) l.
         { induction l as [|x xs IHxs]; auto. cbn.
           rewrite IHxs gen_interp_term_interp_eterm; auto. }
@@ -876,34 +876,33 @@ Section ValidityEquivalence.
       left. rewrite -ls_to_eform_ls_to_form //.
   Qed.
 
-  Fixpoint ls_to_econtext (sko : Skolemization) (Gamma : list EForm) : Con sko :=
+  Fixpoint ls_to_econtext (Gamma : list EForm) : Con :=
     match Gamma with
     | [] => {{ }}
-    | F :: Fs => ls_to_econtext sko Fs ,, [[ F ]]
+    | F :: Fs => ls_to_econtext Fs ,, [[ F ]]
     end.
 
-  (** As we want to avoid defining substitutions for [EForm]s, this theorem is the closest
-      one we can have to a soundness result for the extended syntax. *)
+
   Theorem hasTableau_is_evalid :
     forall (F : EForm) (sko : Skolemization) (Gamma : list EForm) (sigma : Substitution string Term),
-      hasTableau sko (ls_to_econtext sko Gamma ,, Neg [[ F ]]) sigma ->
-      forall M : Model string string,
-        interpret_eform M (subst_to_env M sigma) (EImp (ls_to_eform Gamma) F).
+      @isClosed string Con _ (ls_to_econtext Gamma ,, Neg (translate_EForm F)) ->
+      hasTableau sko (ls_to_econtext Gamma ,, Neg (translate_EForm F)) sigma ->
+      is_evalid (EImp (ls_to_eform Gamma) F).
   Proof.
-    intros ???? htab. apply (hasTableau_sound sko sigma (ls_to_econtext sko Gamma) [[ F ]]) in htab.
+    intros ????? htab. apply (hasTableau_sound sko sigma (ls_to_econtext Gamma) [[ F ]]) in htab; auto.
     unfold is_valid in htab. intros M.
     specialize (htab M).
-    have e : subst_to_env M sigma = extended_environment [] [] (subst_to_env M sigma).
+    have e : empty_env M string = extended_environment [] [] (empty_env M string).
     { now apply funext=>x. }
     rewrite e -gen_translation_equivalidity. cbn.
     cbn in htab. destruct htab as [hGamma | hF].
-    - left. rewrite -subst_commutes_with_env_forms. intro h. apply hGamma.
-      have e' : (translate_EForm_ [] (ls_to_eform Gamma))@[sigma] =
-                  (ls_to_form (forms (ls_to_econtext sko Gamma))@[sigma]).
+    - left. intro h. apply hGamma.
+      have e' : (translate_EForm_ [] (ls_to_eform Gamma)) =
+                  (ls_to_form (ls_to_econtext Gamma)).
       { clear. induction Gamma as [|G Gs IHGs]; cbn in *; try reflexivity.
         now rewrite -IHGs. }
       rewrite -e' //.
-    - right. rewrite -subst_commutes_with_env_forms. exact hF.
+    - right. exact hF.
   Qed.
 End ValidityEquivalence.
 
@@ -959,13 +958,12 @@ Section HasTableauLemmas.
   Context (sko : Skolemization).
 
   Let sko_record := sko_record sko.
-  Let Con := Con sko.
 
   Lemma con_nth_in :
     forall (Gamma : Con) (i : nat) (F : Form),
-      nth_error (forms Gamma) i = Some F -> F \in Gamma.
+      Gamma.(i) = Some F -> F \in Gamma.
   Proof using Type.
-    intros ??? e. unfold in_ctx. revert e. set l := forms Gamma; clearbody l.
+    intros ??? e. unfold in_ctx. revert e. set l := Gamma; clearbody l.
     generalize dependent i. induction l as [|x xs IHxs]; cbn in *;
       intros i e.
     - rewrite nth_error_nil in e; inversion e.
@@ -977,55 +975,54 @@ Section HasTableauLemmas.
   Qed.
 
   Lemma hasTableauBot :
-    forall (Gamma : Con) (sigma : Substitution string Term) (S : SetOfString) (Sf : sko_record) (i : nat),
-      nth_error (forms Gamma) i = Some [[ EBot ]] -> hasTableau_ sko Gamma S Sf sigma.
+    forall (Gamma : Con) (sigma : Substitution string Term) (symbs : sko_record) (i : nat),
+      Gamma.(i) = Some [[ EBot ]] -> hasTableau_ sko Gamma symbs sigma.
   Proof using Type.
-    intros ????? e. apply hasTableauBot.
+    intros ???? e. apply hasTableauBot.
     eapply con_nth_in; eauto.
   Qed.
 
   Lemma hasTableauNegTop :
-    forall (Gamma : Con) (sigma : Substitution string Term) (S : SetOfString) (Sf : sko_record) (i : nat),
-      nth_error (forms Gamma) i = Some [[ ENeg ETop ]] -> hasTableau_ sko Gamma S Sf sigma.
+    forall (Gamma : Con) (sigma : Substitution string Term) (symbs : sko_record) (i : nat),
+      Gamma.(i) = Some [[ ENeg ETop ]] -> hasTableau_ sko Gamma symbs sigma.
   Proof using Type.
-    intros ????? e. eapply hasTableauNegNeg.
+    intros ???? e. eapply hasTableauNegNeg.
     - cbn in e. eapply con_nth_in; eauto.
     - unshelve eapply hasTableauBot; cbn. exact 0. now cbn.
   Qed.
 
   Lemma hasTableauContr :
-    forall (Gamma : Con) (sigma : Substitution string Term) (S : SetOfString) (Sf : sko_record)
+    forall (Gamma : Con) (sigma : Substitution string Term) (symbs : sko_record)
       (i j : nat) (F G : EForm),
-      nth_error (forms Gamma) i = Some [[ F ]] -> nth_error (forms Gamma) j = Some [[ G ]] ->
+      Gamma.(i) = Some [[ F ]] -> Gamma.(j) = Some [[ G ]] ->
       (etranslation_eform (ENeg F))@[sigma] = (etranslation_eform G)@[sigma] ->
-      hasTableau_ sko Gamma S Sf sigma.
+      hasTableau_ sko Gamma symbs sigma.
   Proof using Type.
-    intros ????????? e0 e1.
+    intros ??????? e0 e1 e.
     eapply hasTableauContr; cbn in *.
-    - eapply con_nth_in. exact H.
     - eapply con_nth_in. exact e0.
-    - assumption.
+    - eapply con_nth_in. exact e1.
+    - auto.
   Qed.
 
   Lemma hasTableauNegNeg :
-    forall (Gamma : Con) (sigma : Substitution string Term) (S : SetOfString) (Sf : sko_record)
+    forall (Gamma : Con) (sigma : Substitution string Term) (symbs : sko_record)
       (i : nat) (F : EForm),
-      nth_error (forms Gamma) i = Some [[ ENeg (ENeg F) ]] ->
-      hasTableau_ sko (Gamma ,, [[ F ]]) S Sf sigma ->
-      hasTableau_ sko Gamma S Sf sigma.
+      Gamma.(i) = Some [[ ENeg (ENeg F) ]] ->
+      hasTableau_ sko (Gamma ,, [[ F ]]) symbs sigma ->
+      hasTableau_ sko Gamma symbs sigma.
   Proof using Type.
-    intros ?????? e htab. eapply hasTableauNegNeg; eauto.
+    intros ????? e htab. eapply hasTableauNegNeg; eauto.
     cbn in e; eapply con_nth_in; eauto.
   Qed.
 
   Lemma hasTableauAnd :
-    forall (Gamma : Con) (sigma : Substitution string Term) (S : SetOfString) (Sf : sko_record)
-      (i : nat) (F G : EForm),
-      nth_error (forms Gamma) i = Some [[ EAnd F G ]] ->
-      hasTableau_ sko (Gamma ,, Neg (Neg [[ F ]]) ,, Neg (Neg [[ G ]]) ,, [[ F ]] ,, [[ G ]]) S Sf sigma ->
-      hasTableau_ sko Gamma S Sf sigma.
+    forall (Gamma : Con) (sigma : Substitution string Term) (symbs : sko_record) (i : nat) (F G : EForm),
+      Gamma.(i) = Some [[ EAnd F G ]] ->
+      hasTableau_ sko (Gamma ,, Neg (Neg [[ F ]]) ,, Neg (Neg [[ G ]]) ,, [[ F ]] ,, [[ G ]]) symbs sigma ->
+      hasTableau_ sko Gamma symbs sigma.
   Proof using Type.
-    intros ??????? e htab. eapply hasTableauNegOr.
+    intros ?????? e htab. eapply hasTableauNegOr.
     - cbn in e. eapply con_nth_in; eauto.
     - unshelve eapply hasTableauNegNeg.
       + exact 1.
@@ -1039,25 +1036,24 @@ Section HasTableauLemmas.
   Qed.
 
   Lemma hasTableauNegOr :
-    forall (Gamma : Con) (sigma : Substitution string Term) (S : SetOfString) (Sf : sko_record)
-      (i : nat) (F G : EForm),
-      nth_error (forms Gamma) i = Some [[ ENeg (EOr F G) ]] ->
-      hasTableau_ sko (Gamma ,, [[ ENeg F ]] ,, [[ ENeg G ]]) S Sf sigma ->
-      hasTableau_ sko Gamma S Sf sigma.
+    forall (Gamma : Con) (sigma : Substitution string Term) (symbs : sko_record) (i : nat) (F G : EForm),
+      Gamma.(i) = Some [[ ENeg (EOr F G) ]] ->
+      hasTableau_ sko (Gamma ,, [[ ENeg F ]] ,, [[ ENeg G ]]) symbs sigma ->
+      hasTableau_ sko Gamma symbs sigma.
   Proof using Type.
-    intros ??????? e htab. eapply hasTableauNegOr.
+    intros ?????? e htab. eapply hasTableauNegOr.
     - cbn in e; eapply con_nth_in; eauto.
     - assumption.
   Qed.
 
   Lemma hasTableauNegImp :
-    forall (Gamma : Con) (sigma : Substitution string Term) (S : SetOfString) (Sf : sko_record)
+    forall (Gamma : Con) (sigma : Substitution string Term) (symbs : sko_record)
       (i : nat) (F G : EForm),
-      nth_error (forms Gamma) i = Some [[ ENeg (EImp F G) ]] ->
-      hasTableau_ sko (Gamma ,, [[ ENeg (ENeg F) ]] ,, [[ ENeg G ]] ,, [[ F ]]) S Sf sigma ->
-      hasTableau_ sko Gamma S Sf sigma.
+      Gamma.(i) = Some [[ ENeg (EImp F G) ]] ->
+      hasTableau_ sko (Gamma ,, [[ ENeg (ENeg F) ]] ,, [[ ENeg G ]] ,, [[ F ]]) symbs sigma ->
+      hasTableau_ sko Gamma symbs sigma.
   Proof using Type.
-    intros ??????? e htab. eapply hasTableauNegOr.
+    intros ?????? e htab. eapply hasTableauNegOr.
     - cbn in *; change (Neg [[ F ]]) with ([[ ENeg F ]]) in e; eauto.
     - unshelve eapply hasTableauNegNeg.
       + exact 1.
@@ -1067,49 +1063,42 @@ Section HasTableauLemmas.
   Qed.
 
   Lemma hasTableauOr :
-    forall (Gamma : Con) (sigma : Substitution string Term) (S S1 S2 : SetOfString) (Sf Sf1 Sf2 : sko_record)
-      (i : nat) (F G : EForm),
-      nth_error (forms Gamma) i = Some [[ EOr F G ]] ->
-      hasTableau_ sko (Gamma ,, [[ F ]]) S1 Sf1 sigma ->
-      hasTableau_ sko (Gamma ,, [[ G ]]) S2 Sf2 sigma -> disjoint S1 S2 = true ->
-      eqb S (S1 \union S2) = true -> eqb Sf (join Sf1 Sf2) = true ->
-      hasTableau_ sko Gamma S Sf sigma.
+    forall (Gamma : Con) (sigma : Substitution string Term) (symbs : sko_record) (i : nat) (F G : EForm),
+      Gamma.(i) = Some [[ EOr F G ]] ->
+      hasTableau_ sko (Gamma ,, [[ F ]]) symbs sigma ->
+      hasTableau_ sko (Gamma ,, [[ G ]]) symbs sigma ->
+      hasTableau_ sko Gamma symbs sigma.
   Proof using Type.
-    intros ??????????? e htab1 htab2. rewrite disjoint_are_disjoint.
-    rewrite !eqbIsEq. intros ? -> ->. eapply hasTableauOr.
-    all: eauto.
-    cbn in *; eapply con_nth_in; eauto.
+    intros ?????? e htab1 htab2. eapply hasTableauOr.
+    - eapply con_nth_in; eauto.
+    - assumption.
+    - assumption.
   Qed.
 
   Lemma hasTableauImp :
-    forall (Gamma : Con) (sigma : Substitution string Term) (S S1 S2 : SetOfString) (Sf Sf1 Sf2 : sko_record)
-      (i : nat) (F G : EForm),
-      nth_error (forms Gamma) i = Some [[ EImp F G ]] ->
-      hasTableau_ sko (Gamma ,, [[ ENeg F ]]) S1 Sf1 sigma ->
-      hasTableau_ sko (Gamma ,, [[ G ]]) S2 Sf2 sigma -> disjoint S1 S2 = true ->
-      eqb S (S1 \union S2) = true -> eqb Sf (join Sf1 Sf2) = true ->
-      hasTableau_ sko Gamma S Sf sigma.
+    forall (Gamma : Con) (sigma : Substitution string Term) (symbs : sko_record) (i : nat) (F G : EForm),
+      Gamma.(i) = Some [[ EImp F G ]] ->
+      hasTableau_ sko (Gamma ,, [[ ENeg F ]]) symbs sigma ->
+      hasTableau_ sko (Gamma ,, [[ G ]]) symbs sigma ->
+      hasTableau_ sko Gamma symbs sigma.
   Proof using Type.
-    intros ??????????? e htab1 htab2 hdisjoint e0 e1.
+    intros ?????? e htab1 htab2.
     eapply hasTableauOr.
     1: cbn in *; change (Neg [[ F ]]) with ([[ ENeg F ]]) in e; eassumption.
     all: eauto.
   Qed.
 
   Lemma hasTableauNegAnd :
-    forall (Gamma : Con) (sigma : Substitution string Term) (S S1 S2 : SetOfString) (Sf Sf1 Sf2 : sko_record)
-      (i : nat) (F G : EForm),
-      nth_error (forms Gamma) i = Some [[ ENeg (EAnd F G) ]] ->
-      hasTableau_ sko (Gamma ,, (Or [[ ENeg F ]] [[ ENeg G ]]) ,, [[ ENeg F ]]) S1 Sf1 sigma ->
-      hasTableau_ sko (Gamma ,, (Or [[ ENeg F ]] [[ ENeg G ]]) ,, [[ ENeg G ]]) S2 Sf2 sigma ->
-      disjoint S1 S2 = true -> eqb S (S1 \union S2) = true -> eqb Sf (join Sf1 Sf2) = true ->
-      hasTableau_ sko Gamma S Sf sigma.
+    forall (Gamma : Con) (sigma : Substitution string Term) (symbs : sko_record) (i : nat) (F G : EForm),
+      Gamma.(i) = Some [[ ENeg (EAnd F G) ]] ->
+      hasTableau_ sko (Gamma ,, (Or [[ ENeg F ]] [[ ENeg G ]]) ,, [[ ENeg F ]]) symbs sigma ->
+      hasTableau_ sko (Gamma ,, (Or [[ ENeg F ]] [[ ENeg G ]]) ,, [[ ENeg G ]]) symbs sigma ->
+      hasTableau_ sko Gamma symbs sigma.
   Proof using Type.
-    intros ??????????? e htab1 htab2 e0 e1 hdisjoint. eapply hasTableauNegNeg.
+    intros ?????? e htab1 htab2. eapply hasTableauNegNeg.
     - cbn in *. change (Or (Neg [[ F ]]) (Neg [[ G ]])) with ([[ EOr (ENeg F) (ENeg G) ]]) in e.
       eassumption.
     - unshelve eapply hasTableauOr.
-      1-4: shelve.
       1: exact 0.
       1-2: shelve.
       1: reflexivity.
@@ -1117,18 +1106,16 @@ Section HasTableauLemmas.
   Qed.
 
   Lemma hasTableauEqu :
-    forall (Gamma : Con) (sigma : Substitution string Term) (S S1 S2 : SetOfString) (Sf Sf1 Sf2 : sko_record)
-      (i : nat) (F G : EForm),
-      nth_error (forms Gamma) i = Some [[ (EEqu F G) ]] ->
+    forall (Gamma : Con) (sigma : Substitution string Term) (symbs : sko_record) (i : nat) (F G : EForm),
+      Gamma.(i) = Some [[ (EEqu F G) ]] ->
       hasTableau_ sko (Gamma ,, [[ ENeg (ENeg (EImp F G)) ]] ,, [[ ENeg (ENeg (EImp G F)) ]] ,,
                          [[ EImp F G ]] ,, [[ EImp G F ]] ,, [[ ENeg F ]] ,, [[ ENeg G ]])
-        S1 Sf1 sigma ->
+        symbs sigma ->
       hasTableau_ sko (Gamma ,, [[ ENeg (ENeg (EImp F G)) ]] ,, [[ ENeg (ENeg (EImp G F)) ]] ,,
-                         [[ EImp F G ]] ,, [[ EImp G F ]] ,, [[ G ]] ,, [[ F ]]) S2 Sf2 sigma ->
-      disjoint S1 S2 = true -> eqb S (S1 \union S2) = true -> eqb Sf (join Sf1 Sf2) = true ->
-      hasTableau_ sko Gamma S Sf sigma.
+                         [[ EImp F G ]] ,, [[ EImp G F ]] ,, [[ G ]] ,, [[ F ]]) symbs sigma ->
+      hasTableau_ sko Gamma symbs sigma.
   Proof using Type.
-    intros ??????????? e htab1 htab2 hdisjoint ??. unshelve eapply hasTableauNegOr.
+    intros ?????? e htab1 htab2. unshelve eapply hasTableauNegOr.
     - exact i.
     - exact (ENeg (EImp F G)).
     - exact (ENeg (EImp G F)).
@@ -1142,23 +1129,16 @@ Section HasTableauLemmas.
         * exact (EImp G F).
         * now cbn.
         * unshelve eapply hasTableauOr.
-          1-4: shelve.
-          7-9: eauto.
           -- exact 1.
           -- exact (ENeg F).
           -- exact G.
           -- now cbn.
-          -- replace S1 with (S1 \union empty_set).
-             replace Sf1 with (join Sf1 empty_record).
-             2: apply join_unitr.
-             2: apply empty_unitr.
-             unshelve eapply hasTableauOr.
-             1-4: shelve.
+          -- unshelve eapply hasTableauOr.
              ++ exact 1.
              ++ exact (ENeg G).
              ++ exact F.
              ++ now cbn.
-             ++ eassumption.
+             ++ auto.
              ++ unshelve eapply hasTableauContr.
                 ** exact 0.
                 ** exact 1.
@@ -1167,16 +1147,7 @@ Section HasTableauLemmas.
                 ** now cbn.
                 ** now cbn.
                 ** reflexivity.
-             ++ rewrite disjoint_are_disjoint.
-                eapply empty_disjointr.
-             ++ rewrite eqbIsEq //.
-             ++ rewrite eqbIsEq; reflexivity.
-          -- replace S2 with (empty_set \union S2).
-             replace Sf2 with (join empty_record Sf2).
-             2: apply join_unitl.
-             2: apply empty_unitl.
-             unshelve eapply hasTableauOr.
-             1-4: shelve.
+          -- unshelve eapply hasTableauOr.
              ++ exact 1.
              ++ exact (ENeg G).
              ++ exact F.
@@ -1190,32 +1161,24 @@ Section HasTableauLemmas.
                 ** now cbn.
                 ** reflexivity.
              ++ eassumption.
-             ++ rewrite disjoint_are_disjoint.
-                apply empty_disjointl.
-             ++ rewrite eqbIsEq //.
-             ++ rewrite eqbIsEq; reflexivity.
   Qed.
 
   Lemma hasTableauNegEqu :
-    forall (Gamma : Con) (sigma : Substitution string Term) (S S1 S2 : SetOfString) (Sf Sf1 Sf2 : sko_record)
-      (i : nat) (F G : EForm),
-      nth_error (forms Gamma) i = Some [[ ENeg (EEqu F G) ]] ->
+    forall (Gamma : Con) (sigma : Substitution string Term) (symbs : sko_record) (i : nat) (F G : EForm),
+      Gamma.(i) = Some [[ ENeg (EEqu F G) ]] ->
       hasTableau_ sko (Gamma ,, [[ EOr (ENeg (EImp F G)) (ENeg (EImp G F)) ]] ,, [[ ENeg (EImp F G) ]]
-                         ,, [[ ENeg (ENeg F) ]] ,, [[ ENeg G ]] ,, [[ F ]]) S1 Sf1 sigma ->
+                         ,, [[ ENeg (ENeg F) ]] ,, [[ ENeg G ]] ,, [[ F ]]) symbs sigma ->
       hasTableau_ sko (Gamma ,, [[ EOr (ENeg (EImp F G)) (ENeg (EImp G F)) ]] ,, [[ ENeg (EImp G F) ]]
-                         ,, [[ ENeg (ENeg G) ]] ,, [[ ENeg F ]] ,, [[ G ]]) S2 Sf2 sigma ->
-      disjoint S1 S2 = true -> eqb S (S1 \union S2) = true -> eqb Sf (join Sf1 Sf2) = true ->
-      hasTableau_ sko Gamma S Sf sigma.
+                         ,, [[ ENeg (ENeg G) ]] ,, [[ ENeg F ]] ,, [[ G ]]) symbs sigma ->
+      hasTableau_ sko Gamma symbs sigma.
   Proof using Type.
-    intros ??????????? e htab1 htab2 e1 e2 hdisjoint. unshelve eapply hasTableauNegNeg.
+    intros ?????? e htab1 htab2. unshelve eapply hasTableauNegNeg.
     - exact i.
     - exact (EOr (ENeg (EImp F G)) (ENeg (EImp G F))).
     - now cbn in *.
     - unshelve eapply hasTableauOr.
-      1-4: shelve.
       1: exact 0.
       3: reflexivity.
-      3-5: eauto.
       + unshelve eapply hasTableauNegImp.
         1: exact 0.
         3: reflexivity.
@@ -1227,79 +1190,64 @@ Section HasTableauLemmas.
   Qed.
 
   Lemma hasTableauAll :
-    forall (Gamma : Con) (sigma : Substitution string Term) (S S0 : SetOfString) (Sf : sko_record)
+    forall (Gamma : Con) (sigma : Substitution string Term) (symbs : sko_record)
       (i : nat) (F : EForm) (x : string) (y : string),
-      nth_error (forms Gamma) i = Some [[ EAll x F ]] -> isFresh y (fv Gamma) = true ->
-      mem y (bv_eform F) = false -> S0 = rem y S -> mem y S = true ->
-      hasTableau_ sko (Gamma ,, [[ instantiate_eform x (EVar y) F ]]) S0 Sf sigma ->
-      hasTableau_ sko Gamma S Sf sigma.
+      Gamma.(i) = Some [[ EAll x F ]] ->
+      mem y (bv_eform F) = false -> 
+      hasTableau_ sko (Gamma ,, [[ instantiate_eform x (EVar y) F ]]) symbs sigma ->
+      hasTableau_ sko Gamma symbs sigma.
   Proof using Type.
-    intros ????????? e hfresh hnmem eS hmem htab.
-    have eS0 : S = add y S0.
-    { rewrite eS add_rem; auto.
-      now rewrite -mem_spec. }
-    rewrite eS0. eapply hasTableauAll.
+    intros ??????? e hmem htab. unshelve eapply hasTableauAll.
+    1: exact y.
+    1: shelve.
     - cbn in e. eapply con_nth_in; eauto.
-    - assumption.
     - replace [x] with (List.app [] [x]).
       2: now cbn.
       rewrite (instantiate_eform_commutes_instantiate_form x (EVar y) F []); auto.
       + now cbn.
-      + cbn. now rewrite mem_spec' in hnmem.
+      + cbn. now rewrite mem_spec' in hmem.
   Qed.
 
   Existing Instance fv_ctx.
 
   Lemma hasTableauNegAll :
-    forall (Gamma : Con) (sigma : Substitution string Term) (S : SetOfString) (Sf Sf0 : sko_record)
+    forall (Gamma : Con) (sigma : Substitution string Term) (symbs : sko_record)
       (i : nat) (F : EForm) (x : string) (t : ETerm)
-      (hsko : is_sko (translate_ETerm [] t) (Neg (translate_EForm_ [x] F)) (fv Gamma)
-                (con_sko_record Gamma) = true),
-      nth_error (forms Gamma) i = Some [[ ENeg (EAll x F) ]] ->
-      Sf0 = rem_symbol (symbol sko [[t]] hsko) (translate_EForm_ [x] F) Sf ->
-      in_record (symbol sko [[t]] hsko) Sf ->
+      (hsko : is_sko (translate_ETerm [] t) (Neg (translate_EForm_ [x] F)) (fv Gamma) symbs = true),
+      Gamma.(i) = Some [[ ENeg (EAll x F) ]] ->
       closed_in (fun x s => ~ set_in x s) (bv_eform F) t ->
-      hasTableau_ sko
-        (set_con_sko_record
-           (add_symbol (symbol sko [[t]] hsko) (translate_EForm_ [x] F) (con_sko_record Gamma))
-           (Gamma ,, [[ instantiate_eform x t (ENeg F) ]])) S Sf0 sigma ->
-      hasTableau_ sko Gamma S Sf sigma.
+      hasTableau_ sko (Gamma ,, [[ instantiate_eform x t (ENeg F) ]])
+        (add_symbol (symbol sko [[t]] hsko) (translate_EForm_ [x] F) symbs) sigma ->
+      hasTableau_ sko Gamma symbs sigma.
   Proof using Type.
-    intros ?????????? e0 e1 hin hclosed htab.
-    have e2 : Sf = add_symbol (symbol sko [[t]] hsko) (translate_EForm_ [x] F) Sf0.
-    { rewrite e1. symmetry; now apply add_rem_symbol. }
-    rewrite e2.
-    apply (hasTableauNegAll sko Gamma S Sf0 sigma (translate_EForm_ [x] F) [[ t ]] hsko).
-    - cbn in e0 |- *; eapply con_nth_in; eauto.
-    - have e : (translate_EForm_ [x] (ENeg F)) {0 \to [[t]]} =
-                 [[instantiate_eform x t (ENeg F)]].
+    intros ???????? e hclosed htab.
+    apply (hasTableauNegAll sko Gamma symbs sigma (translate_EForm_ [x] F) [[ t ]] hsko).
+    - cbn in e |- *; eapply con_nth_in; eauto.
+    - have e' : (translate_EForm_ [x] (ENeg F)) {0 \to [[t]]} =
+                  [[instantiate_eform x t (ENeg F)]].
       { replace [x] with (List.app [] [x]).
         2: now cbn.
         rewrite (instantiate_eform_commutes_instantiate_form x t (ENeg F) []); auto; cbn.
         apply closed_in_nil. }
-      rewrite -e in htab. now cbn in htab.
+      rewrite -e' in htab. now cbn in htab.
   Qed.
 
   Lemma hasTableauEx :
-    forall (Gamma : Con) (sigma : Substitution string Term) (S : SetOfString) (Sf Sf0 : sko_record)
+    forall (Gamma : Con) (sigma : Substitution string Term) (symbs : sko_record)
       (i : nat) (F : EForm) (x : string) (t : ETerm)
-      (hsko : is_sko [[ t ]] (Neg (translate_EForm_ [x] (ENeg F)))
-                (fv Gamma) (con_sko_record Gamma) = true),
-      nth_error (forms Gamma) i = Some [[ EEx x F ]] ->
-      Sf0 = rem_symbol (symbol sko [[ t ]] hsko)
-              (translate_EForm_ [x] (ENeg F)) Sf -> in_record (symbol sko [[ t ]] hsko) Sf ->
+      (hsko : is_sko (translate_ETerm [] t) (Neg (Neg (translate_EForm_ [x] F))) (fv Gamma) symbs = true),
+      Gamma.(i) = Some [[ EEx x F ]] ->
       closed_in (fun x s => ~ set_in x s) (bv_eform F) t ->
-      hasTableau_ sko (set_con_sko_record
-                         (add_symbol (symbol sko [[t]] hsko)
-                            (translate_EForm_ [x] (ENeg F)) (con_sko_record Gamma))
-                         (Gamma ,, [[ ENeg (ENeg (instantiate_eform x t F)) ]] ,,
-                            [[ instantiate_eform x t F ]])) S Sf0 sigma ->
-      hasTableau_ sko Gamma S Sf sigma.
+      hasTableau_ sko (Gamma ,, [[ ENeg (ENeg (instantiate_eform x t F)) ]] ,,
+                         [[ instantiate_eform x t F ]])
+        (add_symbol (symbol sko [[t]] hsko) (Neg (translate_EForm_ [x] F)) symbs) sigma ->
+      hasTableau_ sko Gamma symbs sigma.
   Proof using Type.
-    intros ?????????? e0 e1 e2 hclosed htab. eapply hasTableauNegAll.
-    all: eauto.
+    intros ???????? e hclosed htab. eapply hasTableauNegAll.
     Unshelve.
-    3: exact i.
+    4: exact i.
+    4: exact (ENeg F).
+    1: apply e.
     all: eauto.
     change [[instantiate_eform x t (ENeg (ENeg F))]] with
       [[ENeg (ENeg (instantiate_eform x t F))]].
@@ -1311,32 +1259,21 @@ Section HasTableauLemmas.
   Qed.
 
   Lemma hasTableauNegEx :
-    forall (Gamma : Con) (sigma : Substitution string Term) (S S0 : SetOfString) (Sf : sko_record)
+    forall (Gamma : Con) (sigma : Substitution string Term) (symbs : sko_record)
       (i : nat) (F : EForm) (x : string) (y : string),
-      nth_error (forms Gamma) i = Some [[ ENeg (EEx x F) ]] -> isFresh y (fv Gamma) = true ->
-      S0 = rem y S -> mem y S = true -> mem y (bv_eform (ENeg F)) = false ->
+      Gamma.(i) = Some [[ ENeg (EEx x F) ]] ->
+      mem y (bv_eform (ENeg F)) = false ->
       hasTableau_ sko (Gamma ,, [[EAll x (ENeg F)]] ,, [[ instantiate_eform x (EVar y) (ENeg F) ]])
-        S0 Sf sigma -> hasTableau_ sko Gamma S Sf sigma.
+        symbs sigma -> hasTableau_ sko Gamma symbs sigma.
   Proof using Type.
-    intros ????????? e hfresh eS hmem hmem' htab. unshelve eapply hasTableauNegNeg.
+    intros ??????? e hmem htab. unshelve eapply hasTableauNegNeg.
     - exact i.
     - exact (EAll x (ENeg F)).
     - now cbn in e |- *.
     - unshelve eapply hasTableauAll.
-      2: exact 0.
-      5: reflexivity.
-      1-2: shelve.
+      1: exact 0.
+      4: reflexivity.
+      1: shelve.
       all: eauto.
-      have e0 : @fv string Form _ (translate_EForm (EAll x (ENeg F))) =
-                 @fv string Form _ (translate_EForm (ENeg (ENeg (EAll x (ENeg F))))).
-      { reflexivity. }
-      cbn. apply Bool.eq_true_not_negb. rewrite Bool.not_true_iff_false.
-      rewrite (@mem_spec' string SetOfString y (fv (translate_EForm_ [x] F) \union
-                                                  fv (forms Gamma))).
-      apply nth_error_In in e.
-      have els := fv_list_in [[ENeg (EEx x F)]] (forms Gamma) e.
-      cbn in els. rewrite -els.
-      cbn in hfresh. rewrite Bool.negb_true_iff in hfresh.
-      rewrite mem_spec' in hfresh. auto.
   Qed.
 End HasTableauLemmas.
