theories/Proofs.v
@@ -1,5 +1,7 @@
 (** * Proofs: definition of free-variable tableaux proofs. *)
 
+From Stdlib Require Import Classical.
+
 From Tableaux Require Import Semantics.
 From Tableaux Require Import Skolemization.
 From Tableaux Require Import Syntax.
@@ -8,49 +10,30 @@ From Tableaux Require Import Syntax.
 
 (** As we want to keep a [sko_record] in the contexts, contexts get parameterized by
     skolemization instances. *)
-Section Contexts.
-  Context `{set_nat : set nat} {pred func var : Atom} {sko : Skolemization_ pred func var}.
+Section Context.
+  Context `{set_nat : set nat} {pred func var : Atom}.
 
-  Record Con_ :=
-    { forms : list (Form_ pred func var)
-    ; con_sko_record : sko_record sko }.
+  Let Form := Form_ pred func var.
 
-  Definition empty_ctx : Con_ :=
-    {| forms := []
-    ;  con_sko_record := empty_record |}.
+  Definition Con_ := list (Form_ pred func var).
 
-  Definition in_ctx (F : Form_ pred func var) (Gamma : Con_) : Prop :=
-    List.In F (forms Gamma).
+  Definition empty_ctx : Con_ := [].
+  Definition in_ctx (F : Form) (Gamma : Con_) : Prop := List.In F Gamma.
+  Definition extend_ctx (Gamma : Con_) (F : Form) : Con_ := F :: Gamma.
 
-  Definition extend_ctx (Gamma : Con_) (A : Form_ pred func var) : Con_ :=
-    {| forms := A :: forms Gamma
-    ;  con_sko_record := con_sko_record Gamma |}.
+  #[global] Instance fv_ctx : @FV var Con_ := ltac:(typeclasses eauto).
 
-  Fixpoint fv_ctx_ (Gamma : list (Form_ pred func var)) : set_atom var :=
-    match Gamma with
-    | [] => empty_set
-    | F :: Fs => fv F \union fv_ctx_ Fs
-    end.
-
-  #[global] Instance fv_ctx : @FV var Con_ :=
-    fun Gamma => fv_ctx_ (forms Gamma).
-
-  Fixpoint subst_ctx_ (Gamma : list (Form_ pred func var)) (sigma : Substitution var (Term_ func var))
-    : list (Form_ pred func var) :=
+  Fixpoint subst_ctx_ (Gamma : Con_) (sigma : Substitution var (Term_ func var)) : Con_ :=
     match Gamma with
     | [] => []
     | F :: Fs => F@[sigma] :: subst_ctx_ Fs sigma
     end.
 
   #[global] Instance subst_ctx : Subst Con_ (Term_ func var) :=
-    fun Gamma sigma =>
-      {| forms := subst_ctx_ (forms Gamma) sigma
-      ;  con_sko_record := con_sko_record Gamma |}. (* TODO: we probably want to subst this *)
+    subst_ctx_.
 
-  Definition set_con_sko_record (record : sko_record sko) (Gamma : Con_) : Con_ :=
-    {| forms := forms Gamma
-    ;  con_sko_record := record |}.
-End Contexts.
+  Definition ctx_to_form (Gamma : Con_) := ls_to_form Gamma.
+End Context.
 
 Arguments Con_ : clear implicits.
 
@@ -61,6 +44,7 @@ Notation "{{ F }}" := (empty_ctx ,, F).
 Notation "{{ F1 ;; F2 ;; .. ;; Fk }}" :=
   (extend_ctx .. (extend_ctx (extend_ctx empty_ctx F1) F2) .. Fk).
 
+(** ** Definition of tableaux *)
 Section TableauxProofs.
   Context `{set_nat : set nat} {pred func var : Atom} (sko : Skolemization_ pred func var).
 
@@ -68,119 +52,208 @@ Section TableauxProofs.
 
   Let set_var := set_atom var.
   Let set_func := set_atom func.
-  Let Con := Con_ pred func var sko.
+  Let Con := Con_ pred func var.
   Let Term := Term_ func var.
   Let Form := Form_ pred func var.
   Let sko_record := sko_record sko.
 
+  (** We unset the automatic generation of elimination schemes to get a dependent elimination
+      for the predicate [hasTableau_]. *)
+  Unset Elimination Schemes.
   Inductive hasTableau_
-    : Con -> set_var -> sko_record -> Substitution var Term -> Prop :=
+    : Con -> sko_record -> Substitution var Term -> Prop :=
 
   (** Axioms *)
   | hasTableauBot :
-    forall (Gamma : Con) (S : set_var) (Sf : sko_record) (sigma : Substitution var Term),
-      (Bot \in Gamma) -> hasTableau_ Gamma S Sf sigma
+    forall (Gamma : Con) (symbs : sko_record) (sigma : Substitution var Term),
+      (Bot \in Gamma) -> hasTableau_ Gamma symbs sigma
   | hasTableauContr :
-    forall (Gamma : Con) (S : set_var) (Sf : sko_record) (sigma : Substitution var Term)
-      (P P' : Form), (P \in Gamma) -> (P' \in Gamma) -> Neg P@[sigma] = P'@[sigma] -> hasTableau_ Gamma S Sf sigma
+    forall (Gamma : Con) (symbs : sko_record) (sigma : Substitution var Term)
+      (P P' : Form),
+      P \in Gamma -> P' \in Gamma -> Neg P@[sigma] = P'@[sigma] -> hasTableau_ Gamma symbs sigma
 
   (** Alpha rules *)
   | hasTableauNegNeg :
-    forall (Gamma : Con) (S : set_var) (Sf : sko_record) (sigma : Substitution var Term)
-      (F : Form), Neg (Neg F) \in Gamma -> hasTableau_ (Gamma ,, F) S Sf sigma -> hasTableau_ Gamma S Sf sigma
+    forall (Gamma : Con) (symbs : sko_record) (sigma : Substitution var Term) (F : Form),
+      Neg (Neg F) \in Gamma -> hasTableau_ (Gamma ,, F) symbs sigma -> hasTableau_ Gamma symbs sigma
   | hasTableauNegOr :
-    forall (Gamma : Con) (S : set_var) (Sf : sko_record) (sigma : Substitution var Term)
-      (F1 F2 : Form),
-      Neg (Or F1 F2) \in Gamma -> hasTableau_ (Gamma ,, Neg F1 ,, Neg F2) S Sf sigma -> hasTableau_ Gamma S Sf sigma
+    forall (Gamma : Con) (symbs : sko_record) (sigma : Substitution var Term) (F1 F2 : Form),
+      Neg (Or F1 F2) \in Gamma -> hasTableau_ (Gamma ,, Neg F1 ,, Neg F2) symbs sigma -> hasTableau_ Gamma symbs sigma
 
-  (** Beta rule *) (* TODO: JOIN CONDITION IN SKOLEMIZATION *)
+  (** Beta rule *)
   | hasTableauOr :
-    forall (Gamma : Con) (S1 S2 : set_var) (Sf1 Sf2 : sko_record) (sigma : Substitution var Term)
-      (F1 F2 : Form),
-      (Or F1 F2) \in Gamma -> hasTableau_ (Gamma ,, F1) S1 Sf1 sigma -> hasTableau_ (Gamma ,, F2) S2 Sf2 sigma ->
-      are_disjoint S1 S2 -> hasTableau_ Gamma (S1 \union S2) (join Sf1 Sf2) sigma
+    forall (Gamma : Con) (symbs : sko_record) (sigma : Substitution var Term) (F1 F2 : Form),
+      (Or F1 F2) \in Gamma -> hasTableau_ (Gamma ,, F1) symbs sigma -> hasTableau_ (Gamma ,, F2) symbs sigma ->
+      hasTableau_ Gamma symbs sigma
 
   (** Gamma rule *)
   | hasTableauAll :
-    forall (Gamma : Con) (S : set_var) (Sf : sko_record) (sigma : Substitution var Term)
-      (x : var) (F : Form),
-      (All F) \in Gamma -> isFresh x (fv Gamma) = true -> hasTableau_ (Gamma ,, F{0 \to Free x}) S Sf sigma ->
-      hasTableau_ Gamma (add x S) Sf sigma
+    forall (Gamma : Con) (symbs : sko_record) (sigma : Substitution var Term) (x : var) (F : Form),
+      (All F) \in Gamma -> hasTableau_ (Gamma ,, F{0 \to Free x}) symbs sigma ->
+      hasTableau_ Gamma symbs sigma
 
    (** Delta rule *)
   | hasTableauNegAll :
-    forall (Gamma : Con) (S : set_var) (Sf : sko_record) (sigma : Substitution var Term)
-      (F : Form) (t : Term) (Hsko : is_sko t (Neg F) (fv Gamma) (con_sko_record Gamma) = true),
-      (Neg (All F)) \in Gamma -> hasTableau_ (set_con_sko_record
-                                       (add_symbol (symbol sko t Hsko) F (con_sko_record Gamma))
-                                       (Gamma ,, Neg F{0 \to t})) S Sf sigma ->
-      hasTableau_ Gamma S (add_symbol (symbol sko t Hsko) F Sf) sigma.
+    forall (Gamma : Con) (symbs : sko_record) (sigma : Substitution var Term)
+      (F : Form) (t : Term) (Hsko : is_sko t (Neg F) (fv Gamma) symbs = true),
+      (Neg (All F)) \in Gamma ->
+      hasTableau_ (Gamma ,, Neg F{0 \to t}) (add_symbol (symbol sko t Hsko) F symbs) sigma ->
+      hasTableau_ Gamma symbs sigma.
+  Set Elimination Schemes.
+  Scheme hasTableau__ind := Induction for hasTableau_ Sort Prop.
 
   Definition hasTableau (Gamma : Con) (sigma : Substitution var Term) : Prop :=
-    exists (S : set_var) (Sf : sko_record), hasTableau_ Gamma S Sf sigma.
+    hasTableau_ Gamma empty_record sigma.
+
+  (** *** Satisfiability of a tableau *)
+
+  (** A tableau is said satisfiable if there exists a branch such that all the formulas of
+      a branch are satisfiable. We can define it as an inductive predicate. *)
+  Inductive is_tableau_satisfiable (M : Model pred func) (mu : env M var)
+    {Gamma : Con} {symbs : sko_record} {sigma : Substitution var Term} :
+    hasTableau_ Gamma symbs sigma -> Prop :=
+
+  | satisfiable_hasTableauContr :
+    forall (P P' : Form) (hin : P \in Gamma) (hin' : P' \in Gamma) (e : Neg P@[sigma] = P'@[sigma]),
+      [[ M # [] # mu |- ctx_to_form Gamma ]] ->
+      is_tableau_satisfiable M mu (hasTableauContr Gamma symbs sigma P P' hin hin' e)
+
+  | satisfiable_hasTableauNegNeg :
+    forall (F : Form) (hin : Neg (Neg F) \in Gamma) (htab : hasTableau_ (Gamma ,, F) symbs sigma),
+      is_tableau_satisfiable M mu htab ->
+      is_tableau_satisfiable M mu (hasTableauNegNeg Gamma symbs sigma F hin htab)
+
+  | satisfiable_hasTableauNegOr :
+    forall (F1 F2 : Form) (hin : Neg (Or F1 F2) \in Gamma) (htab : hasTableau_ (Gamma ,, Neg F1 ,, Neg F2) symbs sigma),
+      is_tableau_satisfiable M mu htab ->
+      is_tableau_satisfiable M mu (hasTableauNegOr Gamma symbs sigma F1 F2 hin htab)
+
+  | satisfiable_hasTableauOr1 :
+    forall (F1 F2 : Form) (hin : (Or F1 F2) \in Gamma) (htab1 : hasTableau_ (Gamma ,, F1) symbs sigma)
+      (htab2 : hasTableau_ (Gamma ,, F2) symbs sigma),
+      is_tableau_satisfiable M mu htab1 ->
+      is_tableau_satisfiable M mu (hasTableauOr Gamma symbs sigma F1 F2 hin htab1 htab2)
+
+  | satisfiable_hasTableauOr2 :
+    forall (F1 F2 : Form) (hin : (Or F1 F2) \in Gamma) (htab1 : hasTableau_ (Gamma ,, F1) symbs sigma)
+      (htab2 : hasTableau_ (Gamma ,, F2) symbs sigma),
+      is_tableau_satisfiable M mu htab2 ->
+      is_tableau_satisfiable M mu (hasTableauOr Gamma symbs sigma F1 F2 hin htab1 htab2)
+
+  | satisfiable_hasTableauAll :
+    forall (x : var) (F : Form) (hin : (All F) \in Gamma) (htab : hasTableau_ (Gamma ,, F{0 \to Free x}) symbs sigma),
+      is_tableau_satisfiable M mu htab ->
+      is_tableau_satisfiable M mu (hasTableauAll Gamma symbs sigma x F hin htab)
+
+  | satisfiable_hasTableauNegAll :
+    forall (F : Form) (t : Term) (Hsko : is_sko t (Neg F) (fv Gamma) symbs = true)
+      (hin : (Neg (All F)) \in Gamma)
+      (htab : hasTableau_ (Gamma ,, Neg F{0 \to t}) (add_symbol (symbol sko t Hsko) F symbs) sigma),
+      is_tableau_satisfiable M mu htab ->
+      is_tableau_satisfiable M mu (hasTableauNegAll Gamma symbs sigma F t Hsko hin htab).
 End TableauxProofs.
+Arguments is_tableau_satisfiable {_ _ _ _ _} _ _ {_ _ _} _.
 
 (* TODO: structural lemmas, e.g., strengthening, exchange law, (need something else?) *)
 
 Section TableauxSoundness.
   Context `{set_nat : set nat} {pred func var : Atom} (sko : Skolemization_ pred func var).
 
-  Let Con := Con_ pred func var sko.
+  Let Con := Con_ pred func var.
   Let Form := Form_ pred func var.
   Let Term := Term_ func var.
 
-  Lemma subst_ctx_subst_list :
-    forall (Gamma : Con) (sigma : Substitution var Term),
-      (forms Gamma)@[sigma] = forms (Gamma@[sigma]).
-  Proof using Type.
-    intros [l sko_] sigma; cbn. clear sko_; induction l as [|F Fs IHFs]; auto.
-    cbn. f_equal. apply IHFs.
-  Qed.
+  (** We start by showing that if the root formula of a tableau is satisfiable, then this
+      tableau is also satisfiable.
 
+      Note that [Gamma] must be a closed context. *)
+  Lemma hasTableau_satisfiable :
+    forall (M : Model pred func) {Gamma : Con} {symbs : sko_record sko}
+      {sigma : Substitution var Term} (T : hasTableau_ sko Gamma symbs sigma) (mu : env M var),
+      [[ M # [] # mu |- ctx_to_form Gamma ]] ->
+      is_tableau_satisfiable M mu T.
+  Proof.
+    intros ?????? hinterp. induction T.
+    - exfalso. have contra := in_form_list_interp i hinterp.
+      now cbn in contra.
+    - now apply satisfiable_hasTableauContr.
+    - constructor. apply IHT. eapply extend_with_equiv_form; eauto. apply neg_neg_equiv.
+    - constructor. apply IHT. apply interp_list_commute.
+      eapply extend_with_equiv_form; eauto.
+      apply neg_equiv. etransitivity.
+      + apply or_comm.
+      + apply or_equiv; symmetry; apply neg_neg_equiv.
+    - have hinterp' := in_form_list_interp i hinterp.
+      destruct hinterp'.
+      + apply satisfiable_hasTableauOr1. apply IHT1.
+        cbn. intros [hnF1 | hnG]; auto.
+      + apply satisfiable_hasTableauOr2. apply IHT2.
+        cbn. intros [hnF2 | hnG]; auto.
+    - constructor. apply IHT.
+      eapply extend_with_imply_form; eauto.
+      apply instantiate_imply_all. now cbn.
+    - constructor. apply IHT. eapply extend_with_imply_form'.
+      3: apply i.
+      all: auto.
+      exists M, mu. intros hF. apply NNPP in hF.
+      change ([[ M # [] # mu |- F { 0 \to t } ]]) in hF; split.
+      + intros hnAll; apply hnAll. intro c.
+        change [[M # [c] # mu |- F]]. admit.
+      + admit.
+  Admitted.
+
+  (** Of course, no tableau is satisfiable. We start by showing 2 small lemmas: *)
   Lemma in_ctx_in_substituted_ctx :
     forall (Gamma : Con) (F : Form) (sigma : Substitution var Term),
       F \in Gamma -> F@[sigma] \in Gamma@[sigma].
   Proof using Type.
-    intros ???. destruct Gamma as [l sko_]; cbn. clear sko_.
-    induction l as [|G Gs IHGs]; intros Hin; inversion Hin.
+    intros ???. induction Gamma as [|G Gs IHGs]; intros Hin; inversion Hin.
     - rewrite H. cbn. now left.
     - right. now apply IHGs.
   Qed.
 
+  Lemma subst_ctx_subst_list :
+    forall (Gamma : Con) (sigma : Substitution var Term),
+      (ls_to_form Gamma)@[sigma] = ls_to_form (Gamma@[sigma]).
+  Proof using Type.
+    intros; cbn. induction Gamma as [|F Fs IHFs]; auto.
+    cbn. do 3 f_equal. apply IHFs.
+  Qed.
+
+  Lemma hasTableau_not_satisfiable :
+    forall (M : Model pred func)
+      {Gamma : Con} {symbs : sko_record sko} {sigma : Substitution var Term}
+      (T : hasTableau_ sko Gamma symbs sigma), is_tableau_satisfiable M (subst_to_env M sigma) T -> False.
+  Proof using Type.
+    intros ????? hsat. remember (subst_to_env M sigma) as mu. induction hsat.
+    2-7: now apply IHhsat.
+    subst. rewrite -subst_commutes_with_env_forms in H.
+    have h1 : interpret_form_ M [] (empty_env M var) P@[sigma].
+    { eapply in_form_list_interp.
+      - apply in_ctx_in_substituted_ctx; eauto.
+      - rewrite -subst_ctx_subst_list //. }
+    have h2 : interpret_form_ M [] (empty_env M var) (Neg P)@[sigma].
+    { eapply in_form_list_interp.
+      - cbn; rewrite e. apply in_ctx_in_substituted_ctx; eauto.
+      - rewrite -subst_ctx_subst_list //. }
+    cbn in h2. now apply h2.
+  Qed.
+
   Theorem hasTableau_sound :
     forall (sigma : Substitution var Term) (Gamma : Con) (F : Form),
-      hasTableau sko (Gamma ,, Neg F) sigma -> ((forms Gamma)@[sigma] \models F@[sigma]).
-  Proof.
-    intros ??? (S & Sf & htab).
-    rewrite models_iff. replace (Neg F@[sigma] :: (forms Gamma)@[sigma]) with (forms (Gamma ,, Neg F)@[sigma]).
-    2: { rewrite subst_ctx_subst_list. now cbn. }
-    induction htab.
-    - apply in_form_list_models.
-      apply in_ctx_in_substituted_ctx with (sigma := sigma) in H.
-      now cbn in H.
-    - apply in_ctx_in_substituted_ctx with (sigma := sigma) in H0, H.
-      apply models_P_neg_P with (F := P@[sigma]).
-      + now apply in_form_list_models.
-      + apply in_form_list_models. now rewrite H1.
-    - apply extend_with_equiv_form with (F := F0@[sigma]) (G := Neg (Neg F0@[sigma])); auto.
-      + apply neg_neg_equiv.
-      + now apply in_ctx_in_substituted_ctx with (sigma := sigma) in H.
-    - apply extend_with_double_equiv_form with (F1 := Neg F2@[sigma]) (F2 := Neg F1@[sigma])
-                                               (G := Neg (Or F1 F2)@[sigma]); auto.
-      + apply neg_equiv. cbn.
-        rewrite or_comm. apply or_equiv.
-        all: symmetry; apply neg_neg_equiv.
-      + now apply in_ctx_in_substituted_ctx with (sigma := sigma) in H.
-    - apply double_extend_with_equiv_form with (F1 := F1@[sigma]) (F2 := F2@[sigma]) (G := (Or F1 F2)@[sigma]);
-        auto.
-      + reflexivity.
-      + now apply in_ctx_in_substituted_ctx with (sigma := sigma) in H.
-    - apply extend_with_equiv_form' with (F := F0 {0 \to Free x}@[sigma]) (G := (All F0)@[sigma]); auto.
-      + cbn. rewrite form_subst_opening.
-        apply instantiate_imply_all, isLocallyClosed_isLocallyClosed_subst.
-        red. now cbn.
-      + now apply in_ctx_in_substituted_ctx with (sigma := sigma) in H.
-  Admitted.
+      isClosed (Gamma ,, Neg F) ->
+      hasTableau sko (Gamma ,, Neg F) sigma -> Gamma \models F.
+  Proof using Type.
+    intros ??? hclosedGamma htab.
+    rewrite models_iff. intros M. left. intro hsat.
+    have hsat' : interpret_form_ M [] (subst_to_env M sigma) (ls_to_form (Neg F :: Gamma)).
+    { change [[ M # [] # subst_to_env M sigma |- ls_to_form (Neg F :: Gamma) ]].
+      rewrite -subst_commutes_with_env_forms.
+      rewrite isClosed_subst_form; auto.
+      rewrite isClosedList_isClosedFormList //. }
+    clear hsat. eapply hasTableau_satisfiable with (sigma := sigma) (T := htab) in hsat'.
+    eapply hasTableau_not_satisfiable; eauto.
+  Qed.
 End TableauxSoundness.
 
 Module ConcreteProofInstances.
